changes from meeting.

theories/twoLockMSQ_common.v
@@ -1,4 +1,4 @@
-From iris.heap_lang Require Import notation.
+From iris.heap_lang Require Import lang proofmode notation.
 
 (* ===== Linked Lists ===== *)
 
@@ -77,3 +77,170 @@ Proof.
 	- done.
 	- simpl. f_equal. apply IH.
 Qed.
+
+Section All.
+
+Context `{!heapGS Σ}.
+
+Fixpoint All {A} (xs : list A) (f : A -> iProp Σ) : iProp Σ :=
+	match xs with
+	| [] => True
+	| x :: xs' => f x ∗ All xs' f
+	end.
+
+Lemma All_split {A} : forall (xs_1 xs_2 : list A) f,
+	All (xs_1 ++ xs_2) f ∗-∗ All xs_1 f ∗ All xs_2 f.
+Proof.
+	iIntros (xs_1).
+	iInduction (xs_1) as [| x xs'_1] "IH"; iIntros (xs_2 f).
+	- simpl. iSplit; first auto. iIntros "[_ H]". done.
+	- simpl. iSplit.
+	  + iIntros "[Hfx HAll]". iFrame. by iApply "IH".
+	  + iIntros "[[Hfx HAll1] HAll2]". iFrame. iApply "IH". iFrame.
+Qed.
+
+End All.
+
+
+Section isLL.
+
+Context `{!heapGS Σ}.
+
+(* 
+	isLL is short for: 'is Linked List'.
+	isLL_chain states that every node x in xs satisfies 
+		n_in x ↦□ (n_val x, #(n_out x)).
+   	Further, all adjacent pairs, [x ; x'], are connected by x' pointing to x.
+	Example:
+	The list
+	[(l_3_in, v_3, l_3_out); 
+	 (l_2_in, v_2, l_2_out); 
+	 (l_1_in, v_1, l_1_out)] 
+	generates:
+	(v_3, l_3_out) <- l_3_in 	∗	l_3_in <- l_2_out	∗
+	(v_2, l_2_out) <- l_2_in 	∗	l_2_in <- l_1_out	∗
+	(x_1, l_1_out) <- l_1_in
+*)
+
+Fixpoint isLL_chain (xs : list (loc * val * loc) ) : iProp Σ :=
+	match xs with
+	| [] => True
+	| [x] => n_in x ↦□ (n_val x, #(n_out x))
+	| x :: ((x' :: xs'') as xs') =>
+				n_in x ↦□ (n_val x, #(n_out x)) ∗
+				n_out x' ↦□ #(n_in x) ∗
+				isLL_chain xs'
+	end.
+
+(* isLL_chain is persistent for all xs *)
+Global Instance isLL_chain_persistent xs : Persistent (isLL_chain xs).
+Proof.
+	induction xs as [|x [|x' xs']]; apply _.
+Qed.
+
+(* xs defines a linked list, when the tail (the first element of the list) points to NONEV, and all the nodes form a linked list chain. *)
+Definition isLL (xs : list (loc * val * loc) ) : iProp Σ :=
+	match xs with
+	| [] => True
+	| x :: xs' => (n_out x) ↦ NONEV ∗ isLL_chain xs
+	end.
+
+(* Since isLL_chain is persistent, we can always extract it from isLL. *)
+Lemma isLL_and_chain : forall xs,
+	isLL xs -∗
+	isLL xs ∗ isLL_chain xs.
+Proof.
+	iIntros (xs) "HisLLxs".
+	destruct xs as [| x' xs']; first done.
+	unfold isLL.
+	iPoseProof "HisLLxs" as "[Hx'_out #HisLLxs]".
+	iFrame.
+	by iSplit.
+Qed.
+
+(* if two nodes have the same 'in' location, then it is the same node. *)
+Lemma n_in_equal (x y : (loc * val * loc)) :
+	⌜#(n_in x) = #(n_in y)⌝ -∗
+	n_in x ↦□ (n_val x, #(n_out x)) -∗
+	n_in y ↦□ (n_val y, #(n_out y)) -∗
+	⌜x = y⌝.
+Proof.
+	iIntros (Heq_loc) "Hx Hy".
+	simplify_eq.
+	rewrite Heq_loc.
+	iCombine "Hx Hy" gives "[_ %Heq_pair]".
+	simplify_eq.
+	iPureIntro.
+	destruct x as [[lx1 vx] lx2], y as [[ly1 vy] ly2].
+	cbn in *.
+	by subst.
+Qed.
+
+(* If x is an element in an isLL_chain, then it is a node. *)
+Lemma isLL_chain_node : forall xs_1 x xs_2,
+	isLL_chain (xs_1 ++ x :: xs_2) -∗
+	n_in x ↦□ (n_val x, #(n_out x)).
+Proof.
+	iIntros (xs_1 x xs_2) "#HisLL_chain".
+	iInduction xs_1 as [| y xs'_1] "IH".
+	- destruct xs_2.
+	  + done.
+	  + by iDestruct "HisLL_chain" as "(Hx & _ & _)".
+	- iApply "IH". 
+	  destruct xs'_1 as [| y' xs''_1];
+	  iDestruct "HisLL_chain" as "(_ & _ & H)"; done.
+Qed.
+
+Lemma isLL_chain_split : forall xs ys,
+	isLL_chain (xs ++ ys) -∗
+	isLL_chain xs ∗ isLL_chain ys.
+Proof.
+	iIntros (xs ys) "#HisLL_chain_xs_ys".
+	iInduction xs as [|x' xs'] "IH".
+	- by iSplit.
+	- destruct xs' as [| x'' xs''].
+	  + destruct ys as [| y' ys'].
+		* by iSplit.
+		* iDestruct "HisLL_chain_xs_ys" as "(Hx' & Hy'_out & HIsLL_chain_ys')".
+		  fold isLL_chain. iSplit; done.
+	  + iAssert (isLL_chain (x'' :: xs'') ∗ isLL_chain ys)%I as "[IHxs' IHys]".
+	  	{
+			iApply "IH". iDestruct "HisLL_chain_xs_ys" as "(_ & _ & Hchain)"; done.
+		}
+		iSplit; try done.
+		iDestruct "HisLL_chain_xs_ys" as "(Hx'_in & Hx''_out & _)".
+		unfold isLL_chain; auto.
+Qed.
+
+Lemma isLL_chain_agree : forall x y xs xs' ys ys',
+	⌜n_in x = n_in y⌝ -∗
+	isLL_chain (xs ++ [x] ++ xs') -∗
+	isLL_chain (ys ++ [y] ++ ys') -∗
+	⌜x = y⌝.
+Proof.
+	iIntros (x y xs xs' ys ys' Heqn_in_xy) "#HisLL_chainxs #HisLL_chainys".
+	iApply n_in_equal.
+	- iPureIntro. by rewrite Heqn_in_xy.
+	- by iApply (isLL_chain_node xs x xs').
+	- by iApply (isLL_chain_node ys y ys').
+Qed.
+
+Lemma isLL_chain_agree_next : forall x y z ys ys' zs zs',
+	isLL_chain (ys ++ [y ; x] ++ ys') -∗
+	isLL_chain (zs ++ [z ; x] ++ zs') -∗
+	⌜y = z⌝.
+Proof.
+	iIntros (x y z ys ys' zs zs') "#HisLL_chainys #HisLL_chainzs".
+	iPoseProof (isLL_chain_split ys ([y ; x] ++ ys') with "HisLL_chainys") as "[_ HisLL_chain_yxys']".
+	iPoseProof (isLL_chain_split [y ; x] ys' with "HisLL_chain_yxys'") as "[HisLL_chain_yx _]".
+	iPoseProof (isLL_chain_split zs ([z ; x] ++ zs') with "HisLL_chainzs") as "[_ HisLL_chain_zxzs']".
+	iPoseProof (isLL_chain_split [z ; x] zs' with "HisLL_chain_zxzs'") as "[HisLL_chain_zx _]".
+	iClear "HisLL_chainys HisLL_chainzs HisLL_chain_yxys' HisLL_chain_zxzs'".
+	iDestruct "HisLL_chain_yx" as "(#Hy_in_2 & #Hy_out_1 & Hy_in_1)".
+	iDestruct "HisLL_chain_zx" as "(#Hz_in_2 & #Hz_out_1 & Hz_in_1)".
+	iCombine "Hy_out_1 Hz_out_1" gives "[_ %Heq_in]".
+	simplify_eq.
+	iApply n_in_equal; try done. by rewrite Heq_in.
+Qed.
+
+End isLL.
