theories/twoLockMSQ_concurrent_spec.v
@@ -3,8 +3,7 @@ From iris.algebra Require Import excl.
 From iris.bi Require Import derived_laws.
 From iris.heap_lang Require Import lang proofmode notation.
 From iris.heap_lang.lib Require Import lock spin_lock.
-From iris.base_logic.lib Require Import invariants.
-From iris.unstable.heap_lang Require Import interpreter.
+From iris.base_logic.lib Require Import invariants token.
 From MSQueue Require Import twoLockMSQ_impl.
 From MSQueue Require Import twoLockMSQ_common.
 
@@ -14,149 +13,11 @@ Section proofs.
 
 Context `{!heapGS Σ}.
 Context `{!lockG Σ}.
-Context `{!inG Σ (exclR unitO)}.
+Context `{!tokenG Σ}.
 
 Let N := nroot .@ "twoLockMSQ".
 
 (* ===== Concurrent Specification for Two-lock M&S Queue ===== *)
-
-(* 
-	isLL is short for: 'is Linked List'.
-	isLL_chain states that every node x in xs satisfies 
-		n_in x ↦□ (n_val x, #(n_out x)).
-   	Further, all adjacent pairs, [x ; x'], are connected by x' pointing to x.
-	Example:
-	The list
-	[(l_3_in, v_3, l_3_out); 
-	 (l_2_in, v_2, l_2_out); 
-	 (l_1_in, v_1, l_1_out)] 
-	generates:
-	(v_3, l_3_out) <- l_3_in 	∗	l_3_in <- l_2_out	∗
-	(v_2, l_2_out) <- l_2_in 	∗	l_2_in <- l_1_out	∗
-	(x_1, l_1_out) <- l_1_in
-
- *)
-
-Fixpoint isLL_chain (xs : list (loc * val * loc) ) : iProp Σ :=
-	match xs with
-	| [] => True
-	| [x] => n_in x ↦□ (n_val x, #(n_out x))
-	| x :: ((x' :: xs'') as xs') =>
-				n_in x ↦□ (n_val x, #(n_out x)) ∗
-				n_out x' ↦□ #(n_in x) ∗
-				isLL_chain xs'
-	end.
-
-(* isLL_chain is persistent for all xs *)
-Global Instance isLL_chain_persistent xs : Persistent (isLL_chain xs).
-Proof.
-	induction xs as [|x [|x' xs']]; apply _.
-Qed.
-
-(* xs defines a linked list, when the tail (the first element of the list) points to NONEV, and all the nodes form a linked list chain. *)
-Definition isLL (xs : list (loc * val * loc) ) : iProp Σ :=
-	match xs with
-	| [] => True
-	| x :: xs' => (n_out x) ↦ NONEV ∗ isLL_chain xs
-	end.
-
-(* Since isLL_chain is persistent, we can always extract it from isLL. *)
-Lemma isLL_and_chain : forall xs,
-	isLL xs -∗
-	isLL xs ∗ isLL_chain xs.
-Proof.
-	iIntros (xs) "HisLLxs".
-	destruct xs as [| x' xs']; first done.
-	unfold isLL.
-	iPoseProof "HisLLxs" as "[Hx'_out #HisLLxs]".
-	iFrame.
-	by iSplit.
-Qed.
-
-(* if two nodes have the same 'in' location, then it is the same node. *)
-Lemma n_in_equal (x y : (loc * val * loc)) :
-	⌜#(n_in x) = #(n_in y)⌝ -∗
-	n_in x ↦□ (n_val x, #(n_out x)) -∗
-	n_in y ↦□ (n_val y, #(n_out y)) -∗
-	⌜x = y⌝.
-Proof.
-	iIntros (Heq_loc) "Hx Hy".
-	simplify_eq.
-	rewrite Heq_loc.
-	iCombine "Hx Hy" gives "[_ %Heq_pair]".
-	simplify_eq.
-	iPureIntro.
-	destruct x as [[lx1 vx] lx2], y as [[ly1 vy] ly2].
-	cbn in *.
-	by subst.
-Qed.
-
-(* If x is an element in an isLL_chain, then it is a node. *)
-Lemma isLL_chain_node : forall xs_1 x xs_2,
-	isLL_chain (xs_1 ++ x :: xs_2) -∗
-	n_in x ↦□ (n_val x, #(n_out x)).
-Proof.
-	iIntros (xs_1 x xs_2) "#HisLL_chain".
-	iInduction xs_1 as [| y xs'_1] "IH".
-	- destruct xs_2.
-	  + done.
-	  + by iDestruct "HisLL_chain" as "(Hx & _ & _)".
-	- iApply "IH". 
-	  destruct xs'_1 as [| y' xs''_1];
-	  iDestruct "HisLL_chain" as "(_ & _ & H)"; done.
-Qed.
-
-Lemma isLL_chain_split : forall xs ys,
-	isLL_chain (xs ++ ys) -∗
-	isLL_chain xs ∗ isLL_chain ys.
-Proof.
-	iIntros (xs ys) "#HisLL_chain_xs_ys".
-	iInduction xs as [|x' xs'] "IH".
-	- by iSplit.
-	- destruct xs' as [| x'' xs''].
-	  + destruct ys as [| y' ys'].
-		* by iSplit.
-		* iDestruct "HisLL_chain_xs_ys" as "(Hx' & Hy'_out & HIsLL_chain_ys')".
-		  fold isLL_chain. iSplit; done.
-	  + iAssert (isLL_chain (x'' :: xs'') ∗ isLL_chain ys)%I as "[IHxs' IHys]".
-	  	{
-			iApply "IH". iDestruct "HisLL_chain_xs_ys" as "(_ & _ & Hchain)"; done.
-		}
-		iSplit; try done.
-		iDestruct "HisLL_chain_xs_ys" as "(Hx'_in & Hx''_out & _)".
-		unfold isLL_chain; auto.
-Qed.
-
-Lemma isLL_chain_agree : forall x y xs xs' ys ys',
-	⌜n_in x = n_in y⌝ -∗
-	isLL_chain (xs ++ [x] ++ xs') -∗
-	isLL_chain (ys ++ [y] ++ ys') -∗
-	⌜x = y⌝.
-Proof.
-	iIntros (x y xs xs' ys ys' Heqn_in_xy) "#HisLL_chainxs #HisLL_chainys".
-	iApply n_in_equal.
-	- iPureIntro. by rewrite Heqn_in_xy.
-	- by iApply (isLL_chain_node xs x xs').
-	- by iApply (isLL_chain_node ys y ys').
-Qed.
-
-Lemma isLL_chain_agree_next : forall x y z ys ys' zs zs',
-	isLL_chain (ys ++ [y ; x] ++ ys') -∗
-	isLL_chain (zs ++ [z ; x] ++ zs') -∗
-	⌜y = z⌝.
-Proof.
-	iIntros (x y z ys ys' zs zs') "#HisLL_chainys #HisLL_chainzs".
-	iPoseProof (isLL_chain_split ys ([y ; x] ++ ys') with "HisLL_chainys") as "[_ HisLL_chain_yxys']".
-	iPoseProof (isLL_chain_split [y ; x] ys' with "HisLL_chain_yxys'") as "[HisLL_chain_yx _]".
-	iPoseProof (isLL_chain_split zs ([z ; x] ++ zs') with "HisLL_chainzs") as "[_ HisLL_chain_zxzs']".
-	iPoseProof (isLL_chain_split [z ; x] zs' with "HisLL_chain_zxzs'") as "[HisLL_chain_zx _]".
-	iClear "HisLL_chainys HisLL_chainzs HisLL_chain_yxys' HisLL_chain_zxzs'".
-	iDestruct "HisLL_chain_yx" as "(#Hy_in_2 & #Hy_out_1 & Hy_in_1)".
-	iDestruct "HisLL_chain_zx" as "(#Hz_in_2 & #Hz_out_1 & Hz_in_1)".
-	iCombine "Hy_out_1 Hz_out_1" gives "[_ %Heq_in]".
-	simplify_eq.
-	iApply n_in_equal; try done. by rewrite Heq_in.
-Qed.
 
 (* Ghost variable names *)
 Record Qgnames := {γ_Hlock 	: gname;
@@ -170,32 +31,15 @@ Record Qgnames := {γ_Hlock 	: gname;
 				  }.
 
 (* Tokens *)
-Definition TokHlock (g : Qgnames) := own g.(γ_Hlock) (Excl ()).
-Definition TokTlock (g : Qgnames) := own g.(γ_Tlock) (Excl ()).
-Definition TokE (g : Qgnames) := own g.(γ_E) (Excl ()).
-Definition ToknE (g : Qgnames) := own g.(γ_nE) (Excl ()).
-Definition TokD (g : Qgnames) := own g.(γ_D) (Excl ()).
-Definition ToknD (g : Qgnames) := own g.(γ_nD) (Excl ()).
-Definition TokBefore (g : Qgnames) := own g.(γ_Before) (Excl ()).
-Definition TokAfter (g : Qgnames) := own g.(γ_After) (Excl ()).
+Definition TokHlock (g : Qgnames) := token g.(γ_Hlock).
+Definition TokTlock (g : Qgnames) := token g.(γ_Tlock).
+Definition TokE (g : Qgnames) := token g.(γ_E).
+Definition ToknE (g : Qgnames) := token g.(γ_nE).
+Definition TokD (g : Qgnames) := token g.(γ_D).
+Definition ToknD (g : Qgnames) := token g.(γ_nD).
+Definition TokBefore (g : Qgnames) := token g.(γ_Before).
+Definition TokAfter (g : Qgnames) := token g.(γ_After).
 Definition TokUpdated (g : Qgnames) := ((TokBefore g) ∗ (TokAfter g))%I.
-
-Fixpoint All {A} (xs : list A) (f : A -> iProp Σ) : iProp Σ :=
-	match xs with
-	| [] => True
-	| x :: xs' => f x ∗ All xs' f
-	end.
-
-Lemma All_split {A} : forall (xs_1 xs_2 : list A) f,
-	All (xs_1 ++ xs_2) f ∗-∗ All xs_1 f ∗ All xs_2 f.
-Proof.
-	iIntros (xs_1).
-	iInduction (xs_1) as [| x xs'_1] "IH"; iIntros (xs_2 f).
-	- simpl. iSplit; first auto. iIntros "[_ H]". done.
-	- simpl. iSplit.
-	  + iIntros "[Hfx HAll]". iFrame. by iApply "IH".
-	  + iIntros "[[Hfx HAll1] HAll2]". iFrame. iApply "IH". iFrame.
-Qed.
 
 Definition queue_invariant (Ψ : val -> iProp Σ) (l_head l_tail : loc) (Q_γ : Qgnames) : iProp Σ :=
 	∃ xs_v, (* Abstract state *)
@@ -321,20 +165,20 @@ Proof.
 	wp_pures.
 	iMod (pointsto_persist with "Hl_1_in") as "#Hl_1_in".
 	wp_pures.
-	iMod (own_alloc (Excl ()) ) as (γ_D) "Hγ_D"; first done.
+	iMod token_alloc as (γ_D) "Hγ_D".
 	wp_apply (newlock_spec with "Hγ_D").
 	iIntros (hlock γ_Hlock) "Hγ_Hlock".
 	wp_let.
-	iMod (own_alloc (Excl ()) ) as (γ_E) "Hγ_E"; first done.
+	iMod token_alloc as (γ_E) "Hγ_E".
 	wp_apply (newlock_spec with "Hγ_E").
 	iIntros (tlock γ_Tlock) "Hγ_Tlock".
 	wp_let.
 	wp_alloc l_tail as "Hl_tail".
 	wp_alloc l_head as "Hl_head".
-	iMod (own_alloc (Excl ()) ) as (γ_nE) "Hγ_nE"; first done.
-	iMod (own_alloc (Excl ()) ) as (γ_nD) "Hγ_nD"; first done.
-	iMod (own_alloc (Excl ()) ) as (γ_Before) "Hγ_Before"; first done.
-	iMod (own_alloc (Excl ()) ) as (γ_After) "Hγ_After"; first done.
+	iMod token_alloc as (γ_nE) "Hγ_nE".
+	iMod token_alloc as (γ_nD) "Hγ_nD".
+	iMod token_alloc as (γ_Before) "Hγ_Before".
+	iMod token_alloc as (γ_After) "Hγ_After".
 	set (Queue_gnames := {| γ_Hlock := γ_Hlock;
 							γ_Tlock := γ_Tlock;
 							γ_E := γ_E;
